\chapter{Central Simple Algebras}\label{sec:csa}

In this chapter we define central simple algebras. We used some results
in~\cref{sec:unclassified}.

\begin{definition}[Simple Ring] A ring $R$ is simple if the only
  two-sided-ideals of $R$ are ${0}$ and $R$. An algebra is simple if it is
  simple as a ring. \leanok \lean{IsSimpleRing}
\end{definition}

\begin{lemma}
  \label{lem:center-simple-ring}
  Let $A$ be a simple ring, then centre of $A$ is a field. \leanok
  \lean{IsSimpleRing.isField_center}
\end{lemma}
\begin{proof}
  Let $0\ne x$ be an element of centre of $A$. Then $I := \{xy | y\in A\}$ is a
  two-sided-ideal of $A$. Since $0\ne x\in I$, we have that $I = A$. Therefore
  $1 \in I$, hence $x$ is invertible.
\end{proof}

\begin{definition}[Central Algebras]
  Let $R$ be a ring and $A$ an $R$-algebra, we say $A$ is central if and only if
  the centre of $A$ is $R$ \leanok \lean{Algebra.IsCentral}
\end{definition}

\begin{remark}
  Simpleness is invariant under ring isomorphism and centrality is invariant
  under algebra isomorphism.
\end{remark}

\begin{lemma}\label{lem:simple-ring-iff}
  $R$ is a simple ring if and only if any ring homomorphism $f : R \to S$ either
  injective or $S$ is the trivial ring. \leanok
  \lean{IsSimpleRing.iff_injective_ringHom_or_subsingleton_codomain}
\end{lemma}
\begin{proof}
  If $R$ is simple, then the $\ker f$ is either $\{0\}$ or $R$. The former case
  implies that $f$ is injective while the latter case implies that $S$ is the
  trivial ring. Conversely, let $I\subseteq R$ be a two-sided-ideal. Consider
  $\pi: R \to {}^{R}/_{I}$, either $\pi$ is injective implying that $I = \{0\}$
  or that ${}^{R}/_{I}$ is the trivial ring implying that $I = R$.
\end{proof}

\begin{corollary}\label{cor:alghom-bijective-of-dim-eq}
  Assume $R$ is a field. Let $A, B$ be finite dimensional $R$-algebras where $A$
  is simple as well. Then any $R$-algebra homomorphism $f:A\to B$ is bijective
  if $\dim_{R}A=\dim_{R}B$. \leanok
  \lean{bijective_of_dim_eq_of_isCentralSimple}
\end{corollary}
\begin{proof}
  By~\cref{lem:simple-ring-iff}, $f$ is injective. Then
  $\dim_{K}\im f = \dim_{K} B - \dim_{K}\ker f = \dim_{K}B$ meaning that $f$ is
  surjective.
\end{proof}

Let $K$ be a field and $A, B$ be $K$-algebras.
\begin{lemma}
  \label{lem:tensor-central}
  If $A$ and $B$ are central $K$-algebras, $A\otimes_{K}B$ is a central
  $K$-algebra as well. \leanok \lean{IsCentralSimple.TensorProduct.isCentral}
\end{lemma}
\begin{proof}
  Assume $A$ and $B$ are central algebras, then
  by~\cref{cor:center-tensor-tensor}
  $Z\left(A\otimes_{R}B\right)=Z\left(A\right)\otimes_{R}Z\left(B\right)=R\otimes_{R}R=R$.
\end{proof}

\begin{theorem}
  \label{thm:tensor-csa}
  If $A$ is a simple $K$-algebra and $B$ is a central simple $K$-algebra,
  $A\otimes_{K}B$ is a central simple $K$-algebra as well. \leanok
  \lean{IsCentralSimple.TensorProduct.simple}
\end{theorem}
\begin{proof}
  By~\cref{lem:tensor-central}, we need to prove $A\otimes_{K}B$ is a simple
  ring. Denote $f$ as the map $A\to A\otimes_{K}B$. It is sufficient to prove
  that for every two-sided-ideal $I\subseteq A\otimes_{K}B$, we have
  $I = \left\langle f\left(f^{-1}\left(I\right)\right)\right\rangle$. Indeed,
  since $A$ is simple $f^{-1}\left(I\right)$ is either $\left\{0\right\}$ or
  $A$, if it is $\left\{0\right\}$, then $I=\left\{0\right\}$; if it is $A$,
  then $I$ is $A$ as well.

  We will prove that
  $I \le \left\langle f\left(f^{-1}\left(I\right)\right)\right\rangle$, the
  other direction is straightforward. Without loss of generality assume
  $I\ne\left\{0\right\}$. Let $\McA$ be an arbitrary basis of $A$, by
  \cref{lem:expand-tensor-in-basis}, we see that every element
  $x \in A\otimes_{K}B$ can be written as $\sum_{i=0}^{n}\McA_{i}\otimes b_{i}$
  for some natrual number $n$ and some choice of $b_{i}\in B$ and
  $\McA_{i}\in \McA$. Since $I$ is not empty, we see there exists a non-zero
  element $\omega\in I$ such that its expansion
  $\sum_{i=0}^{n}\McA_{i}\otimes b_{i}$ has the minimal $n$. In particular, all
  $b_{i}$ are non-zero and $n\ne0$. We have
  $\omega=\McA_{0}\otimes b_{0}+\sum_{i=1}^{n}\McA_{i}\otimes b_{i}$. Since $B$
  is simple, $1 \in B = \left\langle\langle b_{0} \right\rangle$; hence we write
  $1\in\sum_{j=0}^{m}x_{i}b_{0}y_{i}$ for some $x_{i},y_{i}\in B$. Define
  $\Omega := \sum_{j=0}^{m}(1\otimes x_{i})\omega(1\otimes y_{i})$ which is also
  in $I$. We write
  \[
    \begin{aligned}
      \Omega &= \McA_{0} \otimes \left(\sum_{j=0}^{m}x_{j}b_{0}y_{j}\right) + \sum_{i=1}^{n}\McA_{i}\otimes\left(\sum_{j=0}^{m}x_{j}b_{i}y_{j}\right) \\
             &= \McA_{0}\otimes 1 + \sum_{i=1}^{n}\McA_{i}\otimes\left(\sum_{j=0}^{m}x_{j}b_{i}y_{j}\right)
    \end{aligned}
  \]
  For every $\beta\in B$, we have that
  $\left(1\otimes \beta\right)\Omega - \Omega\left(1\otimes \beta\right)$ is in
  I and is equal to
  \[
    \sum_{i=1}^{n}\McA_{i}\otimes\left(\sum_{j=0}^{m}\beta x_{j}b_{i}y_{j}-x_{j}b_{i}y_{j}\beta\right),
  \]
  which is an expansion of $n-1$ terms, thus
  $\left(1\otimes\beta\right)\Omega-\Omega\left(1\otimes\beta\right)$ must be
  $0$. Hence we conclude that for all $i=1,\dots,n$,
  $\sum_{j=0}^{m}x_{j}b_{i}y_{j}\in Z\left(B\right)=K$. Hence for all
  $i=1,\dots,n$, we find a $\kappa_{i}\in K$ such that
  $\kappa_{i}=\sum_{j=0}^{m}x_{j}b_{i}y_{j}$. Hence we can calculate $\Omega$ as
  \[
    \begin{aligned}
      \Omega &= \McA_{0}\otimes 1 + \sum_{i=1}^{n}\McA_{i}\otimes\left(\sum_{j=0}^{m}\right) \\
             &= \McA_{0}\otimes 1 + \sum_{i=1}^{n}\McA_{i}\otimes\kappa_{i} \\
             &= \left(\McA_{0}+\sum_{i=1}^{n}\kappa_{i}\cdot\McA_{i}\right) \otimes 1
    \end{aligned}.
  \]
  From this, we note that
  $\McA_{0}+\sum_{i}^{n}\kappa_{i}\cdot\McA_{i}\in f^{-1}\left(I\right)$; since
  $A$ is simple, we immediately conclude that $f^{-1}\left(I\right) = A$, once
  we know $\McA_{0}+\sum_{i=1}^{n}\kappa_{i}\cdot \McA_{i}$ is not zero. If it
  is zero, by the fact that $\McA$ is a linearly independent set, we conclude
  that $1,\kappa_{1},\dots,\kappa_{n}$ are all zero; which is a contradiction.
  Since $f^{-1}\left(I\right) = A$, we know
  $\left\langle f\left(f^{-1}I\right)\right\rangle = A \otimes_{K} B$.
\end{proof}

\begin{corollary}\label{lem:cas-basechange}
  Central simple algebras are stable under base change. That is, if $L/K$ is a
  field extension and $D$ is a central simple algebra over $K$, then
  $L\otimes_{K} D$ is central simple over $L$. \leanok
  \lean{IsCentralSimple.baseChange}
\end{corollary}

\begin{proof}
  By~\cref{thm:tensor-csa}, $L\otimes_{K} D$ is simple. Let
  $x\in Z\left(L\otimes_{K}D\right)$, by~\cref{cor:center-tensor-center}, we
  have $x\in Z\left(L\right)\otimes Z\left(D\right)=Z\left(L\right)$. Without
  loss of generality, we can assume that $x = l \otimes d$ is a pure tensor,
  then $l \in Z\left(L\right)$ and $d \in K$. Therefore $x = d\cdot l \in L$.
\end{proof}

%%% Local Variables:
%%% mode: LaTeX
%%% TeX-master: "../print"
%%% End:
